theories/Decidability/UntypedTermination.v
@@ -43,29 +43,432 @@ Proof.
     eapply uconv_sound in Hconv as [? []%algo_conv_sound] ; eauto.
 Qed.
 
+Section GraphInversion.
 
-#[universes(polymorphic)]Definition uconv_str_type
-    (x : uconv_state × term × term)
-    (r : exn errors unit) : Type :=
-  match x,r with
-  | (s,t,u), success _ =>
-      forall (Γ Δ : context) (ρ : Δ ≤ Γ) t' u',
-      t = t'⟨ρ⟩ -> u = u'⟨ρ⟩ -> graph _uconv (s,t',u') ok
-  | (s,t,u), exception e => 
-    forall (Γ Δ : context) (ρ : Δ ≤ Γ) t' u',
-    t = t'⟨ρ⟩ -> u = u'⟨ρ⟩ -> ∑ e', graph _uconv (s,t',u') (exception e')
-  end.
+  Context {I} `{CT : CallTypes I} `{!CallableProps CT} {A B} (f : ∇ (x : A), I ⇒ B x).
 
-Lemma wh_red_str (Γ Δ : context) (ρ : Δ ≤ Γ) t v :
-  graph wh_red t⟨ρ⟩ v ->
-  ∑ v', v = v'⟨ρ⟩ × graph wh_red t v'.
-Proof.
-Admitted.
+  Definition orec_graph'
+    {a} (o : orec I A B (B a)) (b : B a) : Prop :=
+    match o with
+    | _ret x => x = b
+    | _rec x κ => exists v, orec_graph f (f x) v /\ orec_graph f (κ v) b
+    | _call i x κ => exists v, cp_graph i x v /\ orec_graph f (κ v) b
+    | undefined => False
+    end.
 
-Lemma _uconv_str :
-  funrect _uconv (fun _ => True) uconv_str_type.
-Proof.
-Admitted.
+  Definition orec_graph_from {a} {o : orec I A B (B a)} {b}
+    (e : orec_graph f o b) : orec_graph' o b :=
+      match e with
+      | ret_graph _ _ => eq_refl 
+      | rec_graph _ _ _ v _ h h' =>
+          ex_intro _ v (conj h h')
+      | call_graph _ _ _ _ v _ h h' =>
+          ex_intro _ v (conj h h')
+      end.
+
+  Import EqNotations.
+
+  Definition orec_graph_to {a} {o : orec I A B (B a)} {b} :
+    orec_graph' o b -> orec_graph f o b :=
+      match o with
+      | _ret x => fun e => rew e in ret_graph _ _
+      | _rec x κ => fun '(ex_intro _ v (conj h h')) =>
+          rec_graph _ _ _ v _ h h'
+      | _call i x κ => fun '(ex_intro _ v (conj h h')) =>
+          call_graph _ _ _ _ v _ h h'
+      | undefined => fun f => False_rect _ f
+      end.
+
+  Lemma orec_graph_equiv {a} {o : orec I A B (B a)} {b} :
+  orec_graph f o b <-> orec_graph' o b.
+  Proof.
+    split.
+    - apply orec_graph_from.
+    - apply orec_graph_to.
+  Qed.
+
+End GraphInversion.
+
+Section AlgoStr.
+
+  Definition dest_entry_rename (ρ : nat -> nat) (d : dest_entry) : dest_entry :=
+    match d with
+    | eEmptyElim P => eEmptyElim P⟨upRen_term_term ρ⟩
+    | eNatElim P hs hz => eNatElim P⟨upRen_term_term ρ⟩ hs⟨ρ⟩ hz⟨ρ⟩
+    | eApp u => eApp u⟨ρ⟩
+    | eFst => eFst
+    | eSnd => eSnd
+    | eIdElim A x P hr y => eIdElim A⟨ρ⟩ x⟨ρ⟩ P⟨upRen_term_term (upRen_term_term ρ)⟩ hr⟨ρ⟩ y⟨ρ⟩
+    end.
+
+  Lemma map_eq_cons [A B : Type] (f : A -> B) (l : list A) [l' : list B] [b : B] :
+    list_map f l = (b :: l')%list ->
+    ∑ (a : A) (tl : list A),
+    [× l = (a :: tl)%list , f a = b & list_map f tl = l'].
+  Proof.
+    intros e.
+    destruct l ; cbn in * ; inversion e ; subst ; clear e.
+    do 2 eexists ; split ; reflexivity.
+  Qed.
+
+  Lemma zip_rename ρ t π : (zip t π)⟨ρ⟩ = zip t⟨ρ⟩ (list_map (dest_entry_rename ρ) π).
+  Proof.
+    induction π as [|[]] in t |- * ; cbn.
+    1: reflexivity.
+    all: now erewrite IHπ.
+  Qed.
+
+  Lemma red_stack_str :
+    funrect wh_red_stack (fun _ => True)
+      (fun '(t,π) u => forall (ρ : nat -> nat) t' π',
+        t = t'⟨ρ⟩ -> π = List.map (dest_entry_rename ρ) π' -> ∑ u', graph wh_red_stack (t',π') u' × u = u'⟨ρ⟩).
+  Proof.
+    intros ? _ ; cbn.
+    funelim (wh_red_stack _) ; cbn ; try easy.
+    - destruct t1 ; cbn.
+      all: intros ? [] ? [=] ->%eq_sym%List.map_eq_nil ; subst.
+      all: eexists ; split ; [unfold graph ; simp wh_red_stack ; now econstructor|..].
+      all: now bsimpl.
+
+    - intros ? [] ? [=] ->%eq_sym%List.map_eq_nil ; subst.
+      eexists ; split.
+      1: unfold graph ; simp wh_red_stack ; econstructor.
+      reflexivity.
+
+    - split ; [easy|..].
+      intros * IH ? [] ? [=] ([]&?&[? [=]])%eq_sym%map_eq_cons ; subst.
+      edestruct IH as [? []].
+      2: reflexivity.
+      2:{
+        subst.
+        eexists ; split ; [..|reflexivity].
+        unfold graph ; simp wh_red_stack.
+        patch_rec_ret ; econstructor.
+        2: now constructor.
+        eassumption.
+      }
+      now bsimpl.
+
+    - intros ? [] ? [=] ? ; subst.
+      eexists ; split.
+      1: unfold graph ; simp wh_red_stack ; econstructor.
+      now rewrite zip_rename.
+
+    - destruct n0 ; cbn.
+      all: intros ? [] ? [=] ->%eq_sym%List.map_eq_nil ; subst.
+      all: eexists ; split ; [unfold graph ; simp wh_red_stack ; now econstructor|..].
+      all: now bsimpl.
+
+    - split ; [easy|..].
+      intros * IH ? [] ? [=] ([]&?&[? [=]])%eq_sym%map_eq_cons ; subst.
+      edestruct IH as [? []].
+      2: reflexivity.
+      2:{
+        subst.
+        eexists ; split ; [..|reflexivity].
+        unfold graph ; simp wh_red_stack.
+        patch_rec_ret ; econstructor.
+        2: now constructor.
+        eassumption.
+      }
+      now bsimpl.
+
+    - split ; [easy|..].
+      intros * IH ? [] ? [=] ([]&?&[? [=]])%eq_sym%map_eq_cons ; subst.
+      edestruct IH as [? []].
+      1: reflexivity.
+      2:{
+        subst.
+        eexists ; split ; [..|reflexivity].
+        unfold graph ; simp wh_red_stack.
+        patch_rec_ret ; econstructor.
+        2: now constructor.
+        eassumption.
+      }
+      now bsimpl.
+      
+    - intros ? [] ? [=] ->%eq_sym%List.map_eq_nil ; subst.
+      eexists ; split ; [unfold graph ; simp wh_red_stack ; now econstructor|..].
+      now bsimpl.
+
+    - split ; [easy|..].
+      intros * IH ? [] ? [=] ([]&?&[? [=]])%eq_sym%map_eq_cons ; subst.
+      edestruct IH as [? []].
+      1: reflexivity.
+      2:{
+        subst.
+        eexists ; split ; [..|reflexivity].
+        unfold graph ; simp wh_red_stack.
+        patch_rec_ret ; econstructor.
+        2: now constructor.
+        eassumption.
+      }
+      now bsimpl.
+
+    - split ; [easy|..].
+      intros * IH ? [] ? [=] ([]&?&[? [=]])%eq_sym%map_eq_cons ; subst.
+      edestruct IH as [? []].
+      1: reflexivity.
+      2:{
+        subst.
+        eexists ; split ; [..|reflexivity].
+        unfold graph ; simp wh_red_stack.
+        patch_rec_ret ; econstructor.
+        2: now constructor.
+        eassumption.
+      }
+      now bsimpl.
+
+    - intros ? [] ? [=] ->%eq_sym%List.map_eq_nil ; subst.
+      eexists ; split ; [unfold graph ; simp wh_red_stack ; now econstructor|..].
+      now bsimpl.
+ 
+    - split ; [easy|..].
+      intros * IH ? [] ? [=] ([]&?&[? [=]])%eq_sym%map_eq_cons ; subst.
+      edestruct IH as [? []].
+      1: reflexivity.
+      2:{
+        subst.
+        eexists ; split ; [..|reflexivity].
+        unfold graph ; simp wh_red_stack.
+        patch_rec_ret ; econstructor.
+        2: now constructor.
+        eassumption.
+      }
+      now bsimpl.
+
+    - split ; [easy|..].
+      destruct s.
+      all: intros * IH ? [] ? [=] ? ; subst.
+      all: edestruct IH as [? []] ; [reflexivity|..] ; [shelve|..].
+      all: subst.
+      all: eexists ; split ; [..|reflexivity].
+      all: unfold graph ; simp wh_red_stack ; cbn.
+      all: patch_rec_ret ; econstructor ; [..|now constructor].
+      all: eassumption.
+      Unshelve.
+      all: reflexivity.
+  Qed.
+
+  Corollary _wh_red_str :
+    funrect wh_red (fun _ => True) (fun t u => forall (ρ : nat -> nat) t',
+      t = t'⟨ρ⟩ -> ∑ u', graph wh_red t' u' × u = u'⟨ρ⟩).
+  Proof.
+    intros ? _.
+    cbn ; intros ? H ρ t' ->.
+    eapply funrect_graph in H.
+    2: apply red_stack_str.
+    2: easy.
+    edestruct (H ρ t' nil) as [? []].
+    1-2: reflexivity.
+    eexists ; split ; tea.
+    unfold graph.
+    econstructor ; cbn ; tea.
+    now constructor.
+  Qed.
+  
+  Lemma wh_red_str (ρ : nat -> nat) t v :
+    graph wh_red t⟨ρ⟩ v ->
+    ∑ v', v = v'⟨ρ⟩ × graph wh_red t v'.
+  Proof.
+    intros g.
+    eapply funrect_graph in g.
+    2: apply _wh_red_str.
+    2: easy.
+    cbn in g.
+    edestruct g as [? []].
+    1: reflexivity.
+    now easy.
+  Qed.
+
+  Lemma up_inj ρ : ssrfun.injective ρ -> ssrfun.injective (upRen_term_term ρ).
+  Proof.
+    intros H x y e.
+    destruct x,y ; cbn in * ; try congruence.
+    easy.
+  Qed.
+
+  Definition ncan_ne_view1 {N} (w : ~ isCanonical N) : ne_view1 N.
+  Proof.
+    destruct N.
+    all: try solve [destruct w ; econstructor].
+    - now constructor.
+    - eapply (ne_view1_dest _ (eApp _)).
+    - eapply (ne_view1_dest _ (eNatElim _ _ _)).
+    - eapply (ne_view1_dest _ (eEmptyElim _)).
+    - eapply (ne_view1_dest _ eFst).
+    - eapply (ne_view1_dest _ eSnd).
+    - eapply (ne_view1_dest _ (eIdElim _ _ _ _ _)).
+  Defined.
+
+  Lemma ncan_nf_view1 {N} (w : ~ isCanonical N) : build_nf_view1 N = nf_view1_ne (ncan_ne_view1 w).
+  Proof.
+    destruct N ; cbn ; try reflexivity.
+    all: destruct w ; econstructor.
+  Qed.
+
+  Lemma nf_view2_neutral_can t t' :
+    build_nf_view2 t t' = neutrals t t' ->
+    ~ isCanonical t /\ ~ isCanonical t'.
+  Proof.
+    intros Heq.
+    simp build_nf_view2 in Heq.
+    destruct (build_nf_view1 t) as [? [] | | ? [] | | | ] eqn:Heqt ; cbn in Heq.
+    all: destruct (build_nf_view1 t') as [? [] | | ? [] | | | ] eqn:Heqt' ; cbn in Heq.
+    all: try solve [congruence].
+    split.
+    all: now eapply tm_view1_neutral_can.
+  Qed.
+
+  Definition nf_view2_rename (ρ : nat -> nat) {t t' : term} (v : nf_view2 t t') : nf_view2 t⟨ρ⟩ t'⟨ρ⟩ :=
+    match v in nf_view2 x x' return nf_view2 x⟨ρ⟩ x'⟨ρ⟩ with
+    | sorts s s' => sorts s s'
+    | prods A A' B B' => prods A⟨ρ⟩ A'⟨ρ⟩ B⟨upRen_term_term ρ⟩ B'⟨upRen_term_term ρ⟩
+    | nats => nats
+    | emptys => emptys
+    | sigs A A' B B' => sigs A⟨ρ⟩ A'⟨ρ⟩ B⟨upRen_term_term ρ⟩ B'⟨upRen_term_term ρ⟩
+    | ids A A' x x' y y' => ids A⟨ρ⟩ A'⟨ρ⟩ x⟨ρ⟩ x'⟨ρ⟩ y⟨ρ⟩ y'⟨ρ⟩
+    | lams A A' t t' => lams A⟨ρ⟩ A'⟨ρ⟩ t⟨upRen_term_term ρ⟩ t'⟨upRen_term_term ρ⟩
+    | lam_ne A t n' => lam_ne A⟨ρ⟩ t⟨upRen_term_term ρ⟩ n'⟨ρ⟩
+    | ne_lam n A' t' => ne_lam n⟨ρ⟩ A'⟨ρ⟩ t'⟨upRen_term_term ρ⟩
+    | zeros => zeros
+    | succs t t' => succs t⟨ρ⟩ t'⟨ρ⟩
+    | pairs A A' B B' t t' u u' => pairs A⟨ρ⟩ A'⟨ρ⟩ B⟨upRen_term_term ρ⟩ B'⟨upRen_term_term ρ⟩ t⟨ρ⟩ t'⟨ρ⟩ u⟨ρ⟩ u'⟨ρ⟩
+    | pair_ne A B t u n' => pair_ne A⟨ρ⟩ B⟨upRen_term_term ρ⟩ t⟨ρ⟩ u⟨ρ⟩ n'⟨ρ⟩
+    | ne_pair n A' B' t' u' => ne_pair n⟨ρ⟩ A'⟨ρ⟩ B'⟨upRen_term_term ρ⟩ t'⟨ρ⟩ u'⟨ρ⟩
+    | refls A A' x x' => refls A⟨ρ⟩ A'⟨ρ⟩ x⟨ρ⟩ x'⟨ρ⟩
+    | neutrals n n' => neutrals n⟨ρ⟩ n'⟨ρ⟩
+    | mismatch t u => mismatch t⟨ρ⟩ u⟨ρ⟩
+    | anomaly t u => anomaly t⟨ρ⟩ u⟨ρ⟩
+    end.
+
+  Lemma build_nf_view2_rename ρ t t' : build_nf_view2 t⟨ρ⟩ t'⟨ρ⟩ = nf_view2_rename ρ (build_nf_view2 t t').
+  Proof.
+    destruct t, t' ; reflexivity.
+  Qed.
+
+  Definition ne_view2_rename (ρ : nat -> nat) {t t' : term} (v : ne_view2 t t') : ne_view2 t⟨ρ⟩ t'⟨ρ⟩ :=
+    match v in ne_view2 x x' return ne_view2 x⟨ρ⟩ x'⟨ρ⟩ with
+    | ne_rels n n' => ne_rels (ρ n) (ρ n')
+    | ne_apps f u f' u' => ne_apps f⟨ρ⟩ u⟨ρ⟩ f'⟨ρ⟩ u'⟨ρ⟩
+    | ne_nats n P hz hs n' P' hz' hs' => ne_nats
+        n⟨ρ⟩ P⟨upRen_term_term ρ⟩ hz⟨ρ⟩ hs⟨ρ⟩
+        n'⟨ρ⟩ P'⟨upRen_term_term ρ⟩ hz'⟨ρ⟩ hs'⟨ρ⟩
+    | ne_emptys n P n' P' => ne_emptys n⟨ρ⟩ P⟨upRen_term_term ρ⟩ n'⟨ρ⟩ P'⟨upRen_term_term ρ⟩
+    | ne_fsts p p' => ne_fsts p⟨ρ⟩ p'⟨ρ⟩
+    | ne_snds p p' => ne_snds p⟨ρ⟩ p'⟨ρ⟩
+    | ne_ids A x P hr y e A' x' P' hr' y' e' => ne_ids
+      A⟨ρ⟩ x⟨ρ⟩ P⟨upRen_term_term (upRen_term_term ρ)⟩ hr⟨ρ⟩ y⟨ρ⟩ e⟨ρ⟩
+      A'⟨ρ⟩ x'⟨ρ⟩ P'⟨upRen_term_term (upRen_term_term ρ)⟩ hr'⟨ρ⟩ y'⟨ρ⟩ e'⟨ρ⟩
+    | ne_mismatch t u => ne_mismatch t⟨ρ⟩ u⟨ρ⟩
+    | ne_anomaly t u => ne_anomaly t⟨ρ⟩ u⟨ρ⟩
+    end.
+
+  Lemma build_ne_view2_rename ρ t t' : build_ne_view2 t⟨ρ⟩ t'⟨ρ⟩ = ne_view2_rename ρ (build_ne_view2 t t').
+  Proof.
+    destruct t, t' ; reflexivity.
+  Qed.
+
+  #[local] Ltac crush :=
+    repeat match goal with
+      | |- context [build_nf_view1 _] => erewrite ncan_nf_view1 ; cbn
+      | |- forall (_ : exn _ _), _ => intros [] ; cbn
+      | |- ?t = ?t'⟨_⟩ -> _ =>
+            intros _eq ; subst t +
+              (destruct t' ; cbn in _eq ; try solve [congruence] ; inversion _eq ; subst ; clear _eq)
+      | |- forall _ : _, _ => intros ?
+      | |- True => trivial
+      | |- True * _ => split ; [trivial|..]
+      | |- graph _uconv (_, _, _) _ => unfold graph ; simp _uconv uconv_tm_red uconv_ne build_nf_view2 ; cbn
+      | H : _ |- orec_graph ?f (?f ?t) ?r => simple eapply H ; [..|reflexivity|reflexivity]
+      | |- orec_graph _ _ _ => cbn ; patch_rec_ret ; econstructor
+      | |- ssrfun.injective (upRen_term_term _) => apply up_inj
+      | |- ssrfun.injective _ => assumption
+    end.
+
+  Lemma _uconv_str :
+    funrect _uconv (fun _ => True)
+      (fun '(s,t,u) r => forall (ρ : nat -> nat) t' u', ssrfun.injective ρ ->
+        t = t'⟨ρ⟩ -> u = u'⟨ρ⟩ -> graph _uconv (s,t',u') r).
+  Proof.
+    intros ? _ ; cbn.
+    funelim (_uconv _) ; cbn.
+
+    - funelim (uconv_tm _) ; cbn.
+      intros ? red ? red'.
+      split ; [easy|..].
+      intros ? IH ** ; subst.
+      unfold graph ; simp _uconv uconv_tm ; cbn.
+      eapply wh_red_str in red as [? [->]], red' as [? [->]].
+      econstructor.
+      1: eassumption.
+      econstructor.
+      1: eassumption.
+      patch_rec_ret.
+      econstructor ; [..|econstructor].
+      now eapply IH.
+
+    - funelim (uconv_tm_red _) ; cbn.
+      all: match goal with | _ : _ = _ |- _ => shelve | _ => idtac end.
+      all: solve [crush].
+      Unshelve.
+
+      + crush.
+        all: eapply H ; [now eapply up_inj | reflexivity|..].
+        all: now asimpl.
+
+      + crush.
+        all: eapply H ; [now eapply up_inj |idtac|reflexivity].
+        all: now asimpl.
+
+      + crush.
+      
+      + crush.
+
+      + crush.
+
+      + intros.
+        subst.
+        rewrite build_nf_view2_rename in Heq.
+        unfold graph ; simp _uconv uconv_tm_red.
+        destruct (build_nf_view2 _ _) ; cbn in * ; try solve [congruence].
+        now constructor.
+      
+      + easy.
+
+    - funelim (uconv_ne _) ; cbn.
+      1-6,8: solve [crush].
+
+      + intros.
+        subst.
+        rewrite build_ne_view2_rename in Heq.
+        unfold graph ; simp _uconv uconv_ne.
+        destruct (build_ne_view2 _ _) ; cbn in * ; try solve [congruence].
+        now constructor.
+
+      + crush.
+        eapply Nat.eqb_eq in Heq ; subst.
+        match goal with | H : ssrfun.injective _ |- _ => apply H in Heq end.
+        subst.
+        rewrite Nat.eqb_refl ; cbn.
+        now constructor.
+      + crush.
+        eapply Nat.eqb_neq in Heq.
+        rewrite (proj2 (Nat.eqb_neq _ _)) ; cbn ; auto.
+        now constructor.
+
+  Unshelve.
+  all: try solve [apply nf_view2_neutral_can in Heq as [] ; now eintros ?%isCanonical_ren].
+  all: match goal with
+    | |- ~ isCanonical ?t => remember t⟨ρ⟩ as t' in * ; eintros ?%isCanonical_ren
+    end.
+  all: solve [simp build_nf_view2 in Heq ;
+    destruct (build_nf_view1 t') as [? [] | | ? [] | | | ] eqn:Heq' ; subst ; cbn in * ;
+      congruence + (now eapply tm_view1_neutral_can)].
+
+  Qed.
+
+End AlgoStr.
 
 Lemma uconv_expand_ne_eta n n' :
   whne n ->
@@ -87,21 +490,10 @@ Proof.
   apply (orec_graph_rec_inv _uconv) in g as [? [g _]] ; cbn in *.
   simp _uconv uconv_ne to_neutral_diag in g ; cbn in *.
   apply (orec_graph_rec_inv _uconv) in g as [r [g _]] ; cbn in *.
-  unshelve eapply funrect_graph in g.
-  4: apply _uconv_str.
-  2: now cbn.
-  cbn in g.
-  destruct r.
-  - eexists.
-    eapply g.
-    all: unshelve erewrite <- wk1_ren_on ; try reflexivity.
-    1: exact ε.
-    exact (tRel 0).
-  - edestruct g ; cycle -1.
-    now eexists.
-    all: unshelve erewrite <- wk1_ren_on ; try reflexivity.
-    1: exact ε.
-    exact (tRel 0).
+  eapply uconv_wk in g.
+  - now eexists.
+  - intros ??.
+    auto.
 Qed.
 
 Lemma uconv_expand_ne_fst n n' :
